\documentclass[device=normal, lang=cn]{elegantbook}
\usepackage{amsmath}
\usepackage{amssymb}
\usepackage{float}
\usepackage{extarrows}
\usepackage{physics}
\usepackage{mathtools}

\input{math_cmds.tex}

\definecolor{pgcolor}{RGB}{251, 250, 248}
\pagecolor{pgcolor}
\numberwithin{equation}{section}

% \theoremstyle{definition} %
% \newtheorem{property}{Property}[section] %

\title{信号与系统笔记}
\author{FHYQ-Dong}
\date{\today}
\version{1.0}
\cover{images/Note-cover.jpg}
\definecolor{customcoverlinecolor}{RGB}{185, 35, 161}
\colorlet{coverlinecolor}{customcoverlinecolor}


\begin{document}

\maketitle
\frontmatter

\tableofcontents
\mainmatter


\chapter{Z变换}

\section{Z变换的性质}

\subsection{时移性质}
已知$\mathcal{Z}[x(n)] = X(z)$，收敛域$R_1 < \abs{z} < R_2$.
\begin{itemize}
    \item 双边z变换：
    \begin{equation}
        \mathcal{Z}[x(n-m)] = z^{-m}X(z), \quad R_1 < \abs{z} < R_2
    \end{equation}
    \begin{proof}
        \begin{equation}
        \begin{aligned}
            \mathcal{Z}[x(n-m)] &= \sum_{n=-\infty}^{+\infty} x(n-m)z^{-n} = \sum_{k=-\infty}^{+\infty} x(k)z^{-(k+m)} \\
            &= z^{-m}\sum_{k=-\infty}^{+\infty} x(k)z^{-k} = z^{-m}X(z)
        \end{aligned}
        \end{equation}
    \end{proof}
    \item 右边z变换，$m > 0$:
    \begin{align}
        \mathcal{Z}[x(n-m)] &= z^{-m}\qty(X(z) + \sum_{n=-m}^{-1} x(n)z^{-n}), \quad R_1 < \abs{z} < R_2 \\ 
        \mathcal{Z}[x(n+m)] &= z^{m}\qty(X(z) - \sum_{n=1}^{m-1} x(n)z^{-n}), \quad R_1 < \abs{z} < R_2
    \end{align}
    \item 左边z变换，$m > 0$:
    \begin{align}
        \mathcal{Z}[x(n-m)] &= z^{-m}\qty(X(z) - \sum_{n=-m+1}^{0} x(n)z^{-n}), \quad R_1 < \abs{z} < R_2 \\ 
        \mathcal{Z}[x(n+m)] &= z^{m}\qty(X(z) + \sum_{n=0}^{m} x(n)z^{-n}), \quad R_1 < \abs{z} < R_2
    \end{align}
    \begin{proof}
        仅证明右边z变换且$m > 0$的情形，其余类似.
        \begin{equation}
        \begin{aligned}
            \mathcal{Z}[x(n-m)] &= \sum_{n=0}^{+\infty} x(n-m)z^{-n} = \sum_{k=-m}^{+\infty} x(k)z^{-(k+m)} \\
            &= z^{-m}\sum_{k=-m}^{+\infty} x(k)z^{-k} = z^{-m}\qty(X(z) + \sum_{n=-m}^{-1} x(n)z^{-n})
        \end{aligned}
        \end{equation}
    \end{proof}
\end{itemize}


\end{document}
